struggling to add a rewrite rule to unfold adk_mul after bounds have been computed

fiat-rust/src/lib.rs
@@ -24,6 +24,7 @@ pub mod poly1305_32;
 pub mod poly1305_64;
 pub mod secp256k1_dettman_32;
 pub mod secp256k1_dettman_64;
+pub mod secp256k1_dettman_adk_32;
 pub mod secp256k1_montgomery_32;
 pub mod secp256k1_montgomery_64;
 pub mod secp256k1_montgomery_scalar_32;
