src/ExtractionOCaml/with_bedrock2_dettman_multiplication_adk.v
@@ -1,0 +1,4 @@
+Require Import Crypto.Bedrock.Standalone.StandaloneOCamlMain.
+Import Bedrock2Later.
+
+Extraction "src/ExtractionOCaml/with_bedrock2_dettman_multiplication_adk.tmp" DettmanMultiplicationADK.main.
